thys/Real_Time_Deque/RealTimeDeque_Enqueue_Proof.thy
@@ -199,7 +199,7 @@ next
       ?states_stepped = 
       States Left 
           (big_state.Common (state.Idle big_current big_idle))
-          (Small.state.Common (state.Idle small_current small_idle))
+          (small_state.Common (state.Idle small_current small_idle))
       "
        using remaining_steps_idle' invar_stepped remaining_steps_stepped step_n_same
        by (smt (verit) invar_states.elims(2))
@@ -280,7 +280,7 @@ next
       ?states_stepped = 
       States Right 
           (big_state.Common (state.Idle big_current big_idle))
-          (Small.state.Common (state.Idle small_current small_idle))
+          (small_state.Common (state.Idle small_current small_idle))
       "
        using remaining_steps_idle' invar_stepped remaining_steps_stepped step_n_same
        by (smt (verit) invar_states.elims(2))
