thys/Real_Time_Deque/Small_Aux.thy
@@ -8,20 +8,20 @@ text \<open>\<^noindent> Functions:
  \<^descr> \<open>list\<close>: List abstraction of the elements which this end will contain after the transformation is finished. The first phase is not covered, since the elements, which will be transferred from the bigger deque end are not known yet.
  \<^descr> \<open>list_current\<close>: List abstraction of the elements currently in this deque end.\<close>
 
-fun list :: "'a state \<Rightarrow> 'a list" where
+fun list :: "'a small_state \<Rightarrow> 'a list" where
   "list (Common common) = Common_Aux.list common"
 | "list (Reverse2 (Current extra _ _ remained) aux big new count) =
   extra @ (take_rev (remained - (count + size big)) aux) @ (rev (Stack_Aux.list big) @ new)"
 
-fun list_current :: "'a state \<Rightarrow> 'a list" where
+fun list_current :: "'a small_state \<Rightarrow> 'a list" where
   "list_current (Common common) = Common_Aux.list_current common"
 | "list_current (Reverse2 current _ _ _ _) = Current_Aux.list current"
 | "list_current (Reverse1 current _ _) = Current_Aux.list current"
 
-instantiation state::(type) invar
+instantiation small_state::(type) invar
 begin
 
-fun invar_state :: "'a state \<Rightarrow> bool" where
+fun invar_small_state :: "'a small_state \<Rightarrow> bool" where
   "invar (Common state) = invar state"
 | "invar (Reverse2 current auxS big newS count) = (
    case current of Current _ _ old remained \<Rightarrow>
@@ -42,10 +42,10 @@ fun invar_state :: "'a state \<Rightarrow> bool" where
 instance..
 end
 
-instantiation state::(type) size
+instantiation small_state::(type) size
 begin
 
-fun size_state :: "'a state \<Rightarrow> nat" where
+fun size_small_state :: "'a small_state \<Rightarrow> nat" where
   "size (Common state) = size state"
 | "size (Reverse2 current _ _ _ _) = min (size current) (size_new current)"
 | "size (Reverse1 current _ _) = min (size current) (size_new current)"
@@ -53,10 +53,10 @@ fun size_state :: "'a state \<Rightarrow> nat" where
 instance..
 end
 
-instantiation state::(type) size_new
+instantiation small_state::(type) size_new
 begin
 
-fun size_new_state :: "'a state \<Rightarrow> nat" where
+fun size_new_small_state :: "'a small_state \<Rightarrow> nat" where
   "size_new (Common state) = size_new state"
 | "size_new (Reverse2 current _ _ _ _) = size_new current"
 | "size_new (Reverse1 current _ _) = size_new current"
